subst

dev/lf/dot_rec.v
@@ -209,6 +209,7 @@ with fv_defs(ds: defs) : vars :=
   end.
 
 Definition fv_ctx_types(G: ctx): vars := (fv_in_values (fun T => fv_typ T) G).
+Definition fv_sto_vals(s: sto): vars := (fv_in_values (fun T => fv_val T) s).
 
 (* ###################################################################### *)
 (** ** Operational Semantics *)
@@ -399,7 +400,7 @@ Ltac gather_vars :=
   let A := gather_vars_with (fun x : vars      => x         ) in
   let B := gather_vars_with (fun x : var       => \{ x }    ) in
   let C := gather_vars_with (fun x : ctx       => (dom x) \u (fv_ctx_types x)) in
-  let D := gather_vars_with (fun x : sto       => dom x     ) in
+  let D := gather_vars_with (fun x : sto       => dom x   \u (fv_sto_vals x)) in
   let E := gather_vars_with (fun x : avar      => fv_avar  x) in
   let F := gather_vars_with (fun x : trm       => fv_trm   x) in
   let G := gather_vars_with (fun x : val       => fv_val   x) in
@@ -714,13 +715,19 @@ Qed.
 (* ###################################################################### *)
 (** ** Substitution *)
 
-Definition subst_avar (z: var) (u: var) (a: avar) : avar :=
-  match a with
-  | avar_b i => avar_b i
-  | avar_f x => (avar_f (If x = z then u else x))
+Definition subst_fvar (z: var) (u: fvar) (v: fvar) : fvar :=
+  match v with
+  | in_sto x => in_sto x
+  | in_ctx x => (If x = z then u else in_ctx x)
   end.
 
-Fixpoint subst_typ (z: var) (u: var) (T: typ) { struct T } : typ :=
+Definition subst_avar (z: var) (u: fvar) (a: avar) : avar :=
+  match a with
+  | avar_b i => avar_b i
+  | avar_f v => avar_f (subst_fvar z u v)
+  end.
+
+Fixpoint subst_typ (z: var) (u: fvar) (T: typ) { struct T } : typ :=
   match T with
   | typ_top        => typ_top
   | typ_bot        => typ_bot
@@ -730,13 +737,13 @@ Fixpoint subst_typ (z: var) (u: var) (T: typ) { struct T } : typ :=
   | typ_bnd T      => typ_bnd (subst_typ z u T)
   | typ_all T U    => typ_all (subst_typ z u T) (subst_typ z u U)
   end
-with subst_dec (z: var) (u: var) (D: dec) { struct D } : dec :=
+with subst_dec (z: var) (u: fvar) (D: dec) { struct D } : dec :=
   match D with
   | dec_typ L T U => dec_typ L (subst_typ z u T) (subst_typ z u U)
   | dec_trm L U => dec_trm L (subst_typ z u U)
   end.
 
-Fixpoint subst_trm (z: var) (u: var) (t: trm) : trm :=
+Fixpoint subst_trm (z: var) (u: fvar) (t: trm) : trm :=
   match t with
   | trm_var x        => trm_var (subst_avar z u x)
   | trm_val v        => trm_val (subst_val z u v)
@@ -744,31 +751,38 @@ Fixpoint subst_trm (z: var) (u: var) (t: trm) : trm :=
   | trm_app x1 x2    => trm_app (subst_avar z u x1) (subst_avar z u x2)
   | trm_let t1 t2    => trm_let (subst_trm z u t1) (subst_trm z u t2)
   end
-with subst_val (z: var) (u: var) (v: val) : val :=
+with subst_val (z: var) (u: fvar) (v: val) : val :=
   match v with
   | val_new T ds     => val_new (subst_typ z u T) (subst_defs z u ds)
   | val_lambda T t   => val_lambda (subst_typ z u T) (subst_trm z u t)
   end
-with subst_def (z: var) (u: var) (d: def) : def :=
+with subst_def (z: var) (u: fvar) (d: def) : def :=
   match d with
   | def_typ L T => def_typ L (subst_typ z u T)
   | def_trm L t => def_trm L (subst_trm z u t)
   end
-with subst_defs (z: var) (u: var) (ds: defs) : defs :=
+with subst_defs (z: var) (u: fvar) (ds: defs) : defs :=
   match ds with
   | defs_nil => defs_nil
   | defs_cons rest d => defs_cons (subst_defs z u rest) (subst_def z u d)
   end.
 
-Definition subst_ctx (z: var) (u: var) (G: ctx) : ctx := map (subst_typ z u) G.
+Definition subst_ctx (z: var) (u: fvar) (G: ctx) : ctx := map (subst_typ z u) G.
+Definition subst_sto (z: var) (u: fvar) (s: sto) : sto := map (subst_val z u) s.
 
 (* ###################################################################### *)
 (** ** Lemmas for var-by-var substitution *)
 
+Lemma subst_fresh_fvar: forall x y,
+  (forall v: fvar, x \notin fv_fvar v -> subst_fvar x y v = v).
+Proof.
+  intros. unfold fv_fvar in *. destruct* v. simpl. case_var*. simpls. notin_false.
+Qed.
+
 Lemma subst_fresh_avar: forall x y,
   (forall a: avar, x \notin fv_avar a -> subst_avar x y a = a).
 Proof.
-  intros. destruct* a. simpl. case_var*. simpls. notin_false.
+  intros. destruct* a. simpl. f_equal. apply* subst_fresh_fvar.
 Qed.
 
 Lemma subst_fresh_typ_dec: forall x y,
@@ -778,8 +792,8 @@ Proof.
   intros x y. apply typ_mutind; intros; simpls; f_equal*. apply* subst_fresh_avar.
 Qed.
 
-Definition subst_fresh_typ(x y: var) := proj1 (subst_fresh_typ_dec x y).
-Definition subst_fresh_dec(x y: var) := proj2 (subst_fresh_typ_dec x y).
+Definition subst_fresh_typ x y := proj1 (subst_fresh_typ_dec x y).
+Definition subst_fresh_dec x y := proj2 (subst_fresh_typ_dec x y).
 
 Lemma subst_fresh_trm_val_def_defs: forall x y,
   (forall t : trm , x \notin fv_trm  t  -> subst_trm  x y t  = t ) /\
@@ -791,10 +805,10 @@ Proof.
     (apply* subst_fresh_avar || apply* subst_fresh_typ_dec).
 Qed.
 
-Definition subst_fresh_trm (x y: var) := proj41 (subst_fresh_trm_val_def_defs x y).
-Definition subst_fresh_val (x y: var) := proj42 (subst_fresh_trm_val_def_defs x y).
-Definition subst_fresh_def (x y: var) := proj43 (subst_fresh_trm_val_def_defs x y).
-Definition subst_fresh_defs(x y: var) := proj44 (subst_fresh_trm_val_def_defs x y).
+Definition subst_fresh_trm  x y := proj41 (subst_fresh_trm_val_def_defs x y).
+Definition subst_fresh_val  x y := proj42 (subst_fresh_trm_val_def_defs x y).
+Definition subst_fresh_def  x y := proj43 (subst_fresh_trm_val_def_defs x y).
+Definition subst_fresh_defs x y := proj44 (subst_fresh_trm_val_def_defs x y).
 
 Lemma invert_fv_ctx_types_push: forall x z T G,
   x \notin fv_ctx_types (G & z ~ T) -> x \notin fv_typ T /\ x \notin (fv_ctx_types G).
@@ -808,6 +822,21 @@ Proof.
   do 2 rewrite LibList.fold_right_cons in *.
   simpl in *.
   apply notin_union in N. exact N.
+Qed.
+
+Lemma fv_ctx_types_push: forall x z T G,
+  x \notin fv_typ T -> x \notin (fv_ctx_types G) ->
+  x \notin fv_ctx_types (G & z ~ T).
+Proof.
+  introv A B.
+  unfold fv_ctx_types in *.
+  unfold fv_in_values in *.
+  rewrite <- cons_to_push in *.
+  rewrite values_def in *.
+  unfold LibList.map in *.
+  do 2 rewrite LibList.fold_right_cons in *.
+  simpl in *.
+  apply notin_union. split; assumption.
 Qed.
 
 Lemma subst_fresh_ctx: forall x y G,
@@ -824,16 +853,61 @@ Proof.
     reflexivity.
 Qed.
 
-Definition subst_fvar(x y z: var): var := If z = x then y else z.
+Lemma fv_ctx_types_binds: forall x z T G,
+  x \notin fv_ctx_types G -> binds z T G ->
+  x \notin fv_typ T.
+Proof.
+  intros.
+  unfold fv_ctx_types in *.
+  eapply fv_in_values_binds; eassumption.
+Qed.
+
+Lemma invert_fv_sto_vals_push: forall x z v s,
+  x \notin fv_sto_vals (s & z ~ v) -> x \notin fv_val v /\ x \notin (fv_sto_vals s).
+Proof.
+  introv N.
+  unfold fv_sto_vals in *.
+  unfold fv_in_values in *.
+  rewrite <- cons_to_push in *.
+  rewrite values_def in *.
+  unfold LibList.map in *.
+  do 2 rewrite LibList.fold_right_cons in *.
+  simpl in *.
+  apply notin_union in N. exact N.
+Qed.
+
+Lemma subst_fresh_sto: forall x y s,
+  x \notin fv_sto_vals s -> subst_sto x y s = s.
+Proof.
+  intros x y.
+  apply (env_ind (fun s => x \notin fv_sto_vals s -> subst_sto x y s = s)).
+  + intro N. unfold subst_sto. apply map_empty.
+  + intros G z T IH N.
+    apply invert_fv_sto_vals_push in N. destruct N as [N1 N2].
+    unfold subst_sto in *. rewrite map_push.
+    rewrite (IH N2).
+    rewrite subst_fresh_val.
+    reflexivity.
+    apply N1.
+Qed.
+
+Lemma fv_sto_vals_binds: forall x z v s,
+  x \notin fv_sto_vals s -> binds z v s ->
+  x \notin fv_val v.
+Proof.
+  intros.
+  unfold fv_sto_vals in *.
+  eapply fv_in_values_binds; eassumption.
+Qed.
 
 Lemma subst_open_commute_avar: forall x y u,
   (forall a: avar, forall n: Datatypes.nat,
     subst_avar x y (open_rec_avar n u a)
-    = open_rec_avar n (subst_fvar x y u) (subst_avar  x y a)).
+    = open_rec_avar n (subst_fvar x y u) (subst_avar x y a)).
 Proof.
   intros. unfold subst_fvar, subst_avar, open_avar, open_rec_avar. destruct a.
   + repeat case_if; auto.
-  + case_var*.
+  + reflexivity.
 Qed.
 
 (* "open and then substitute" = "substitute and then open" *)
@@ -900,7 +974,7 @@ Qed.
 (* "Introduce a substitution after open": Opening a term t with a var u is the
    same as opening t with x and then replacing x by u. *)
 Lemma subst_intro_trm: forall x u t, x \notin (fv_trm t) ->
-  open_trm u t = subst_trm x u (open_trm x t).
+  open_trm u t = subst_trm x u (open_trm (in_ctx x) t).
 Proof.
   introv Fr. unfold open_trm. rewrite* subst_open_commute_trm.
   destruct (@subst_fresh_trm_val_def_defs x u) as [Q _]. rewrite* (Q t).
@@ -908,7 +982,7 @@ Proof.
 Qed.
 
 Lemma subst_intro_val: forall x u v, x \notin (fv_val v) ->
-  open_val u v = subst_val x u (open_val x v).
+  open_val u v = subst_val x u (open_val (in_ctx x) v).
 Proof.
   introv Fr. unfold open_trm. rewrite* subst_open_commute_val.
   destruct (@subst_fresh_trm_val_def_defs x u) as [_ [Q _]]. rewrite* (Q v).
@@ -916,7 +990,7 @@ Proof.
 Qed.
 
 Lemma subst_intro_defs: forall x u ds, x \notin (fv_defs ds) ->
-  open_defs u ds = subst_defs x u (open_defs x ds).
+  open_defs u ds = subst_defs x u (open_defs (in_ctx x) ds).
 Proof.
   introv Fr. unfold open_trm. rewrite* subst_open_commute_defs.
   destruct (@subst_fresh_trm_val_def_defs x u) as [_ [_ [_ Q]]]. rewrite* (Q ds).
@@ -924,7 +998,7 @@ Proof.
 Qed.
 
 Lemma subst_intro_typ: forall x u T, x \notin (fv_typ T) ->
-  open_typ u T = subst_typ x u (open_typ x T).
+  open_typ u T = subst_typ x u (open_typ (in_ctx x) T).
 Proof.
   introv Fr. unfold open_typ. rewrite* subst_open_commute_typ.
   destruct (@subst_fresh_typ_dec x u) as [Q _]. rewrite* (Q T).
@@ -932,24 +1006,32 @@ Proof.
 Qed.
 
 Lemma subst_intro_dec: forall x u D, x \notin (fv_dec D) ->
-  open_dec u D = subst_dec x u (open_dec x D).
+  open_dec u D = subst_dec x u (open_dec (in_ctx x) D).
 Proof.
   introv Fr. unfold open_trm. rewrite* subst_open_commute_dec.
   destruct (@subst_fresh_typ_dec x u) as [_ Q]. rewrite* (Q D).
   unfold subst_fvar. case_var*.
 Qed.
 
-Lemma subst_undo_avar: forall x y,
-  (forall a, y \notin fv_avar a -> (subst_avar y x (subst_avar x y a)) = a).
+Lemma subst_undo_fvar: forall x y,
+  (forall v, y \notin fv_fvar v -> (subst_fvar y (in_ctx x) (subst_fvar x (in_ctx y) v)) = v).
 Proof.
-  intros. unfold subst_avar, subst_fvar, open_avar, open_rec_avar; destruct a.
+  intros. unfold subst_fvar, subst_fvar; destruct v.
   + reflexivity.
-  + unfold fv_avar in H. assert (y <> v) by auto. repeat case_if; reflexivity.
+  + unfold fv_fvar in H. assert (y <> v) by auto. repeat case_if; reflexivity.
+Qed.
+
+Lemma subst_undo_avar: forall x y,
+  (forall a, y \notin fv_avar a -> (subst_avar y (in_ctx x) (subst_avar x (in_ctx y) a)) = a).
+Proof.
+  intros. unfold subst_avar; destruct a.
+  + reflexivity.
+  + f_equal. apply* subst_undo_fvar.
 Qed.
 
 Lemma subst_undo_typ_dec: forall x y,
-   (forall T , y \notin fv_typ  T  -> (subst_typ  y x (subst_typ  x y T )) = T )
-/\ (forall D , y \notin fv_dec  D  -> (subst_dec  y x (subst_dec  x y D )) = D ).
+   (forall T , y \notin fv_typ  T  -> (subst_typ y (in_ctx x) (subst_typ  x (in_ctx y) T )) = T )
+/\ (forall D , y \notin fv_dec  D  -> (subst_dec y (in_ctx x) (subst_dec  x (in_ctx y) D )) = D ).
 Proof.
   intros.
   apply typ_mutind; intros; simpl; unfold fv_typ, fv_dec in *; f_equal*.
@@ -957,10 +1039,10 @@ Proof.
 Qed.
 
 Lemma subst_undo_trm_val_def_defs: forall x y,
-   (forall t , y \notin fv_trm  t  -> (subst_trm  y x (subst_trm  x y t )) = t )
-/\ (forall v , y \notin fv_val  v  -> (subst_val  y x (subst_val  x y v )) = v )
-/\ (forall d , y \notin fv_def  d  -> (subst_def  y x (subst_def  x y d )) = d )
-/\ (forall ds, y \notin fv_defs ds -> (subst_defs y x (subst_defs x y ds)) = ds).
+   (forall t , y \notin fv_trm  t  -> (subst_trm  y (in_ctx x) (subst_trm  x (in_ctx y) t )) = t )
+/\ (forall v , y \notin fv_val  v  -> (subst_val  y (in_ctx x) (subst_val  x (in_ctx y) v )) = v )
+/\ (forall d , y \notin fv_def  d  -> (subst_def  y (in_ctx x) (subst_def  x (in_ctx y) d )) = d )
+/\ (forall ds, y \notin fv_defs ds -> (subst_defs y (in_ctx x) (subst_defs x (in_ctx y) ds)) = ds).
 Proof.
   intros.
   apply trm_mutind; intros; simpl; unfold fv_trm, fv_val, fv_def, fv_defs in *; f_equal*;
@@ -968,23 +1050,31 @@ Proof.
 Qed.
 
 Lemma subst_typ_undo: forall x y T,
-  y \notin fv_typ T -> (subst_typ y x (subst_typ x y T)) = T.
+  y \notin fv_typ T -> (subst_typ y (in_ctx x) (subst_typ x (in_ctx y) T)) = T.
 Proof.
   apply* subst_undo_typ_dec.
 Qed.
 
 Lemma subst_trm_undo: forall x y t,
-  y \notin fv_trm t -> (subst_trm y x (subst_trm x y t)) = t.
+  y \notin fv_trm t -> (subst_trm y (in_ctx x) (subst_trm x (in_ctx y) t)) = t.
 Proof.
   apply* subst_undo_trm_val_def_defs.
+Qed.
+
+Lemma subst_idempotent_fvar: forall x y,
+  (forall v, (subst_fvar x y (subst_fvar x y v)) = (subst_fvar x y v)).
+Proof.
+  intros. unfold subst_fvar; destruct v.
+  + reflexivity.
+  + case_if; eauto; destruct y; eauto; case_if; eauto.
 Qed.
 
 Lemma subst_idempotent_avar: forall x y,
   (forall a, (subst_avar x y (subst_avar x y a)) = (subst_avar x y a)).
 Proof.
-  intros. unfold subst_avar, subst_fvar, open_avar, open_rec_avar; destruct a.
+  intros. unfold subst_avar; destruct a.
   + reflexivity.
-  + repeat case_if; reflexivity.
+  + f_equal. apply* subst_idempotent_fvar.
 Qed.
 
 Lemma subst_idempotent_typ_dec: forall x y,
